theories/L/AbstractMachines/FlatPro/Computable/Compile.v
@@ -1,0 +1,124 @@
+From Undecidability.L Require Import L Tactics.LTactics Prelim.LoopSum Functions.LoopSum.
+From Undecidability.L.Datatypes Require Import LSum LBool LNat Lists.
+
+From Undecidability.L.AbstractMachines  Require Import FlatPro.Programs Computable.LPro.
+
+(*
+fix compile (s : term) : list Tok :=
+  match s with
+  | # x => [varT x]
+  | app s0 t => compile s0 ++ compile t ++ [appT]
+  | lam s0 => lamT :: compile s0 ++ [retT]
+  end 
+ *)
+
+Local Definition c__size := 22.
+
+Lemma compile_enc_size s: size (enc (compile s)) <= size s * c__size.
+Proof.
+  rewrite size_list. unfold enc;cbn.
+  induction s;cbn [compile].
+  all:repeat (cbn [map size sumn token_enc];autorewrite with list).
+  all:ring_simplify.
+  rewrite size_nat_enc.
+  all:repeat first[rewrite <- IHs1,<- IHs2 | rewrite <- IHs]. all:ring_simplify.
+  all:unfold c__size;nia.
+Qed.
+
+Definition compileTR' '(stack,res) : (list (term + bool) * list Tok) + list Tok :=
+  match stack with
+    [] => inr res
+  | inr true :: stack => inl (stack, retT::res)
+  | inr false :: stack => inl (stack, appT::res)
+  | inl s::stack =>
+    match s with
+      var n => inl (stack,varT n :: res)
+    | app s t => inl (inl s::inl t::inr false::stack,res)
+    | lam s => inl (inl s::inr true::stack,lamT::res)
+    end
+  end.
+
+Fixpoint compileTR'_fuel (s:term) : nat :=
+  match s with
+    var _ => 1
+  | app s t => 1 + (compileTR'_fuel s + (compileTR'_fuel t + 1))
+  | lam s => 1 + (compileTR'_fuel s + 1)
+  end.
+
+Lemma compileTR'_correct stack res s k:
+  loopSum (compileTR'_fuel s + k) compileTR' (inl s::stack,res)
+  = loopSum k compileTR' (stack,rev (compile s) ++ res).
+Proof.
+  induction s in res,stack,k |- *.
+  all:cbn.
+  -reflexivity.
+  -rewrite <- !Nat.add_assoc. cbn.
+   erewrite IHs1, IHs2. cbn. now autorewrite with list.
+  -rewrite <- !Nat.add_assoc. rewrite IHs. cbn. autorewrite with list. easy. 
+Qed.
+                       
+Lemma compileTR_correct s:
+  loopSum (compileTR'_fuel s + 1) compileTR' ([inl s],[]) = Some (rev (compile s)). 
+Proof.
+  rewrite compileTR'_correct. cbn. now autorewrite with list.
+Qed.
+
+Definition c__compileTR' := 32.
+Instance termT_compileTR' : computableTime' compileTR'
+                                           (fun x _ => (c__compileTR',tt)).
+Proof.
+  extract. unfold c__compileTR'. solverec. 
+Qed.
+
+Lemma compileTR'_fuel_leq_size s : compileTR'_fuel s <= size s * 2.
+Proof.
+  induction s;cbn [size compileTR'_fuel];try Lia.lia.
+Qed.
+  
+
+From Undecidability Require Import Functions.UnboundIteration.
+
+
+Local Definition c1 := (c__compileTR' * 2 + 44).
+Local Definition c2 := 59.
+Definition time_compile x := c1*x +c2.
+
+Instance termT_compile : computableTime' compile (fun s _ => (time_compile (size s),tt)).
+Proof.
+  evar (time : nat -> nat). [time]:intros n0.
+  set (f:=(fun s : term => rev (compile s))) in .
+  eassert (computableTime' f (fun s _ => (time (size s),tt))).
+  eexists.
+  eapply computesTime_timeLeq.
+  2:{ unshelve (eapply uiter_total_instanceTime with (1 := compileTR_correct) (preprocessT:=(fun _ _ => (6,tt)))).
+      4:{ extract. solverec. }
+      2:{ apply termT_compileTR'. }
+  }
+  {
+    intros s _;cbn [fst snd]. split. 2:easy.
+    evar (c1 : nat). evar (c2 : nat).
+    evar (perItem : term + bool -> nat).
+    erewrite uiterTime_bound_recRel with (iterT := fun _ '(stack,_) => (sumn (map perItem stack) + 41))
+                                         (P:= fun n x => True).
+    4:easy. 3:reflexivity.
+    2:{ intros n ([|[[]|[]]]&res) _.
+        all:cbn. 
+        easy. all:split;[easy|].
+        all:ring_simplify.
+        [perItem]:refine (fun c => match c with
+                                | inr _ => c1 + c__compileTR'
+                                | inl s => (c2 + c__compileTR') * compileTR'_fuel s
+                                end).
+        all:cbn [perItem compileTR'_fuel].
+        [c1]:exact 9. all:subst c1. 4-5:nia.
+        all:ring_simplify. [c2]:exact 9.
+        all:subst c2;nia.
+    } subst c1 c2.
+    cbn [sumn map perItem]. rewrite compileTR'_fuel_leq_size. set (size s). ring_simplify. unfold time. reflexivity.
+  }
+  eapply computableTimeExt with (x:= fun s => rev (f s)).
+  1:{ cbn;unfold f;intro. now autorewrite with list. }
+  extract. solverec. unfold f, time. rewrite rev_length, length_compile_leq.
+  ring_simplify. 
+  unfold time_compile, c1,c2. (*ring_simplify*) nia.
+Qed.
