theories/L/Complexity/Problems/TMGenNP_fixed_mTM.v
@@ -1,0 +1,20 @@
+From Undecidability.TM Require Import TM.
+From Undecidability.L.TM Require Import TMflat TMflatEnc TMflatFun TMEncoding TapeDecode TMunflatten TMflatFun.
+From Undecidability.L.Datatypes Require Import LNat LProd Lists.
+From Undecidability.L.Complexity Require Import NP LinTimeDecodable ONotation.
+From Undecidability.L Require Import Tactics.LTactics Functions.Decoding TMflatFun.
+From Undecidability Require Import L.Functions.EqBool.
+From Undecidability Require Import L.Datatypes.LNat.
+
+
+Definition TMGenNP_fixed_mTM' (sig : finType) `{registered sig} n (M : mTM sig (S n)) : Vector.t (tape sig) n * nat * nat -> Prop :=
+  fun '(ts, maxSize, steps) =>
+    exists t1, sizeOfTape t1 <= maxSize /\ exists f, loopM (initc M (t1:::ts)) steps = Some f.
+
+Definition HaltsOrDiverges_fixed_mTM (sig : finType) `{registered sig} n (M : mTM sig (S n)) : Vector.t (tape sig) n * nat * nat -> Prop :=
+  fun '(ts, maxSize, steps) =>
+    forall t1, sizeOfTape t1 <= maxSize -> forall k f, loopM (initc M (t1:::ts)) steps = Some f -> k <= steps.
+
+Definition GenNPHalt_fixed_mTM (sig : finType) `{registered sig} n (M : mTM sig (S n))
+  := restrictBy (HaltsOrDiverges_fixed_mTM M) (TMGenNP_fixed_mTM' M).
+
