theories/L/Complexity/Reductions/TMGenNP/LMGenNPHalt.v
@@ -1,0 +1,90 @@
+From Undecidability.L Require Import Tactics.LTactics Prelim.MoreList Prelim.MoreBase.
+From Undecidability.L.Complexity Require Import NP Synthetic Monotonic GenNPHalt.
+
+From Undecidability.L Require Import LM_heap_def LM_heap_correct LBool ResourceMeasures Compile LNat LTerm Compile.
+
+(** The halting formulation of the generic NP-complete problem for the abstract machine executing L-terms. 
+This is usefull as we have a Turing machine that simulates this abstract machine. *)
+
+Definition initLMGen s c : (list (nat*list Tok)*list (nat*list Tok)*list (option ((nat * list Tok) * nat)))
+  := ([(0,s++c++[appT])],[],[]).
+
+Section fixX.
+  Context (X:Type) `{R__X : registered X}.
+  
+  Definition LMGenNPHalt' : list Tok*nat*nat -> Prop :=
+    fun '(P, maxSize, k (*in unary*)) =>
+      exists (c:X), size (enc c) <= maxSize /\ (exists sigma' k', k' <= k /\ evaluatesIn step k' (initLMGen P (compile (enc c))) sigma').
+
+  Definition LMHaltsOrDiverges : list Tok*nat*nat -> Prop :=
+    fun '(P, maxSize, steps (*in unary*)) =>
+      (exists s, P = compile s /\ proc s)
+      /\ forall (c : X), size (enc c) <= maxSize -> forall k sigma', evaluatesIn step k (initLMGen P (compile (enc c))) sigma' -> k <= steps.
+
+  Definition LMGenNPHalt := restrictBy LMHaltsOrDiverges LMGenNPHalt'.
+End fixX.
+
+Arguments LMGenNPHalt : clear implicits.
+Arguments LMGenNPHalt _ {_}.
+
+Lemma polyRed_GenNPHalt_to_LMGenNPHalt (X:Type) `{R__X : registered X}:
+  GenNPHalt X ⪯p LMGenNPHalt X.
+Proof.
+  evar (f__steps : nat -> nat). [f__steps]:intros n0.
+  pose (f := (fun '(s, maxSize, steps) => (compile s,maxSize : nat, f__steps steps))).
+  eapply reducesPolyMO_intro_restrictBy with (f:=f).
+  2:{
+    intros [[s' maxSize] steps]. cbn - [GenNPHalt' LMGenNPHalt'].
+    intros (cs&Hsize). assert (lambda s') as [s0 eq] by Lproc. set (s:=lam s0) in *. subst s'.
+    split.
+    -split. easy.
+     intros c H k sigma' R__M. unfold initLMGen in R__M.
+     eapply soundnessTime with (s:=(L.app s (@enc _ R__X c))) in R__M as (g&H'&t&n&eq__sigma&Rs%timeBS_evalIn&_&eq). 2:Lproc.
+     subst k. apply Hsize in Rs. rewrite Rs. unfold f__steps. reflexivity. easy. 
+    -apply Morphisms_Prop.ex_iff_morphism. intros c.
+     apply Morphisms_Prop.and_iff_morphism_obligation_1. easy.
+     split.
+     +intros (?&(?&?&Ev)%evalLe_evalIn). eapply timeBS_evalIn,completenessTime in Ev. 2:Lproc.
+      destruct Ev as (g&Heap&?&Rs).
+      eexists _,_. split. 2:split. 2:exact Rs. now cbn; lia. now intros ? ?.
+     +intros (?&?&?&R__M).
+      eapply soundnessTime with (s:=(L.app s (@enc _ R__X c))) in R__M as (g&H'&t&n&eq__sigma&Rs%timeBS_evalIn&_&eq). 2:Lproc.
+      eexists. eapply evalIn_evalLe. 2:easy. cbn in H;nia.
+  }
+  subst f__steps;cbn beta in f.
+  evar (time : nat -> nat). [time]:intros n0.
+  exists time.
+  { unfold f. extract.
+    solverec.
+    set (n0:=(size (enc (a0, b0, b)))).
+    eassert (b <= n0) as ->.
+    {subst n0. rewrite !LProd.size_prod;cbn [fst snd]. now rewrite size_nat_enc_r at 1. }
+    unfold time_compile.
+    eassert (size a0 <= n0) as ->.
+    {subst n0. rewrite !LProd.size_prod;cbn [fst snd]. now rewrite LTerm.size_term_enc_r at 1. }
+    unfold time. reflexivity.
+  }
+  1,2:now unfold time;smpl_inO.
+  {unfold f. evar (resSize : nat -> nat). [resSize]:intros n0. eexists resSize.
+   {intros [[x mSize] steps].
+    set(n0:=size (enc (x, mSize, steps))).
+    rewrite !LProd.size_prod;cbn [fst snd].
+    setoid_rewrite size_nat_enc at 2.
+    eassert (steps <= n0) as ->.
+    {subst n0. rewrite !LProd.size_prod;cbn [fst snd]. now rewrite size_nat_enc_r at 1. }
+    eassert (size (enc mSize) <= n0) as ->.
+    {subst n0. rewrite !LProd.size_prod;cbn [fst snd]. easy. }
+    rewrite compile_enc_size.
+    eassert (size x <= n0) as ->.
+    {subst n0. rewrite !LProd.size_prod;cbn [fst snd]. now rewrite size_term_enc_r at 1. }
+    unfold resSize. reflexivity.
+   }
+   1,2:unfold resSize;smpl_inO.
+  }
+Qed.
+
+Lemma NPhard_LMGenNPHalt X__cert `{R__cert : registered X__cert}:
+  canEnumTerms X__cert->  NPhard (LMGenNPHalt X__cert).
+Proof.
+  intros ?%NPhard_GenNPHalt. now eapply (red_NPhard polyRed_GenNPHalt_to_LMGenNPHalt).
+Qed.
